theories/typing/fixpoint.v
@@ -1,0 +1,67 @@
+From lrust.lifetime Require Import definitions.
+From lrust.typing Require Export type bool.
+
+Section fixpoint.
+  Context `{typeG Σ}.
+
+  Global Instance type_inhabited : Inhabited type := populate bool.
+
+  Context (T : type → type) `{Contractive T}.
+
+  (* FIXME : Contrarily to the rule on paper, these rules are
+     coinductive: they let one assume [ty] is [Copy]/[Send]/[Sync] to
+     prove that [T ty] is [Copy]/[Send]/[Sync]. *)
+  Global Instance fixpoint_copy :
+    (∀ `(!Copy ty), Copy (T ty)) → Copy (fixpoint T).
+  Proof.
+    intros ?. apply fixpoint_ind.
+    - intros ??[[EQsz%leibniz_equiv EQown]EQshr].
+      specialize (λ tid vl, EQown tid vl). specialize (λ κ tid l, EQshr κ tid l).
+      simpl in *=>-[Hp Hsh]; (split; [intros ??|intros ???]).
+      + revert Hp. by rewrite /PersistentP -EQown.
+      + intros F l q. rewrite -EQsz -EQshr. setoid_rewrite <-EQown. auto.
+    - exists bool. apply _.
+    - done.
+    - intros c Hc. split.
+      + intros tid vl. apply uPred.equiv_entails, equiv_dist=>n.
+        by rewrite conv_compl uPred.always_always.
+      + intros κ tid E F l q ? ?.
+        apply uPred.entails_equiv_and, equiv_dist=>n. etrans.
+        { apply equiv_dist, uPred.entails_equiv_and, (copy_shr_acc κ tid E F)=>//.
+          by rewrite -conv_compl. }
+        do 2 f_equiv; first by rewrite conv_compl. do 8 (f_contractive || f_equiv).
+        * by rewrite -conv_compl.
+        * destruct n. done. by setoid_rewrite conv_compl.
+        * by rewrite -conv_compl.
+        * f_equiv. f_contractive. unfold dist_later. destruct n=>//.
+          by setoid_rewrite conv_compl.
+  Qed.
+
+  Global Instance fixpoint_send :
+    (∀ `(!Send ty), Send (T ty)) → Send (fixpoint T).
+  Proof.
+    intros ?. apply fixpoint_ind.
+    - intros ?? EQ ????. by rewrite -EQ.
+    - exists bool. apply _.
+    - done.
+    - intros c Hc ???. apply uPred.entails_equiv_and, equiv_dist=>n.
+      rewrite conv_compl. apply equiv_dist, uPred.entails_equiv_and; apply Hc.
+  Qed.
+
+  Global Instance fixpoint_sync :
+    (∀ `(!Sync ty), Sync (T ty)) → Sync (fixpoint T).
+  Proof.
+    intros ?. apply fixpoint_ind.
+    - intros ?? EQ ?????. by rewrite -EQ.
+    - exists bool. apply _.
+    - done.
+    - intros c Hc ????. apply uPred.entails_equiv_and, equiv_dist=>n.
+      rewrite conv_compl. apply equiv_dist, uPred.entails_equiv_and; apply Hc.
+  Qed.
+
+  Lemma fixpoint_unfold_eqtype E L : eqtype E L (fixpoint T) (T (fixpoint T)).
+  Proof.
+    unfold eqtype, subtype, type_incl. setoid_rewrite <-fixpoint_unfold.
+    split; iIntros "_ _ _"; (iSplit; first done); iSplit; iIntros "!#*$".
+  Qed.
+End fixpoint.
